disk-betree/AsyncMain.dfy
@@ -1,0 +1,219 @@
+include "MapSpec.dfy"
+include "CrashSafe.dfy"
+include "AsyncDiskModel.dfy"
+include "../lib/NativeTypes.dfy"
+
+module DiskTypes {
+  import opened NativeTypes
+  type LBA = uint64
+  type ByteSector = seq<byte>
+}
+
+abstract module Main {
+  import ADM : AsyncDiskModel
+  import D = AsyncDisk
+
+  import MS = MapSpec
+  import CrashSafeMap
+  import opened NativeTypes
+  import opened Options
+  import DiskTypes
+  import UI
+
+  type UIOp = ADM.M.UIOp
+
+  // impl defined stuff
+
+  type Constants // impl defined
+  type HeapState // impl defined (heap state)
+  function HeapSet(hs: HeapState) : set<object>
+
+  predicate Inv(k: Constants, hs: HeapState)
+    reads HeapSet(hs)
+  function Ik(k: Constants): ADM.M.Constants
+  function I(k: Constants, hs: HeapState): ADM.M.Variables
+    requires Inv(k, hs)
+    reads HeapSet(hs)
+  function ILBA(lba: LBA) : ADM.M.LBA
+
+  predicate ValidSector(sector: Sector)
+
+  function ISector(sector: Sector) : ADM.M.Sector
+    requires ValidSector(sector)
+
+  method InitState() returns (k: Constants, hs: HeapState)
+    ensures Inv(k, hs)
+
+  // DiskInterface
+
+  function method BlockSize() : uint64 { 8*1024*1024 }
+
+  type LBA = DiskTypes.LBA
+  type Sector = DiskTypes.ByteSector
+
+  type DiskOp = D.DiskOp<LBA, Sector>
+  type ReqRead = D.ReqRead<LBA>
+  type ReqWrite = D.ReqWrite<LBA, Sector>
+  type RespRead = D.RespRead<Sector>
+  type RespWrite = D.RespWrite
+
+  predicate ValidReqRead(reqRead: ReqRead) { true }
+  predicate ValidReqWrite(reqWrite: ReqWrite) { ValidSector(reqWrite.sector) }
+  predicate ValidRespRead(respRead: RespRead) { ValidSector(respRead.sector) }
+  predicate ValidRespWrite(respWrite: RespWrite) { true }
+  predicate ValidDiskOp(dop: DiskOp)
+  {
+    match dop {
+      case ReqReadOp(id, reqRead) => true
+      case ReqWriteOp(id, reqWrite) => ValidSector(reqWrite.sector)
+      case RespReadOp(id, respRead) => ValidSector(respRead.sector)
+      case RespWriteOp(id, respWrite) => true
+      case NoDiskOp => true
+    }
+  }
+
+  class DiskIOHandler {
+    method {:axiom} write(lba: LBA, sector: array<byte>) returns (id : D.ReqId)
+    modifies this;
+    requires diskOp() == D.NoDiskOp;
+    requires sector.Length == BlockSize() as int
+    requires ValidSector(sector[..])
+    ensures diskOp() == D.ReqWriteOp(id, D.ReqWrite(lba, sector[..]));
+
+    method {:axiom} read(lba: LBA) returns (id: D.ReqId)
+    modifies this
+    requires diskOp() == D.NoDiskOp
+    ensures diskOp() == D.ReqReadOp(id, D.ReqRead(lba))
+
+    function {:axiom} diskOp() : DiskOp
+    reads this
+    ensures ValidDiskOp(diskOp())
+
+    predicate initialized()
+    reads this
+    {
+      diskOp() == D.NoDiskOp
+    }
+  }
+
+  class DiskIOWriteResult {
+    method {:axiom} getResult() returns (id : D.ReqId)
+    modifies this;
+    ensures diskOp() == D.RespWriteOp(id, D.RespWrite)
+
+    function {:axiom} diskOp() : DiskOp
+    reads this
+    ensures ValidDiskOp(diskOp())
+    ensures diskOp().RespWriteOp?
+  }
+
+  class DiskIOReadResult {
+    method {:axiom} getResult() returns (id : D.ReqId, sector: array<byte>)
+    modifies this;
+    ensures sector.Length == BlockSize() as int
+    ensures ValidSector(sector[..])
+    ensures diskOp() == D.RespReadOp(id, D.RespRead(sector[..]))
+
+    function {:axiom} diskOp() : DiskOp
+    reads this
+    ensures ValidDiskOp(diskOp())
+    ensures diskOp().RespReadOp?
+  }
+
+  function IReqRead(reqRead: ReqRead) : ADM.M.ReqRead
+  requires ValidReqRead(reqRead)
+  {
+    D.ReqRead(ILBA(reqRead.lba))
+  }
+  function IReqWrite(reqWrite: ReqWrite) : ADM.M.ReqWrite
+  requires ValidReqWrite(reqWrite)
+  {
+    D.ReqWrite(ILBA(reqWrite.lba), ISector(reqWrite.sector))
+  }
+  function IRespRead(respRead: RespRead) : ADM.M.RespRead
+  requires ValidRespRead(respRead)
+  {
+    D.RespRead(ISector(respRead.sector))
+  }
+  function IRespWrite(respWrite: RespWrite) : ADM.M.RespWrite
+  requires ValidRespWrite(respWrite)
+  {
+    D.RespWrite
+  }
+
+  function IDiskOp(diskOp: DiskOp) : ADM.M.DiskOp
+  requires ValidDiskOp(diskOp)
+  {
+    match diskOp {
+      case ReqReadOp(id, reqRead) => D.ReqReadOp(id, IReqRead(reqRead))
+      case ReqWriteOp(id, reqWrite) => D.ReqWriteOp(id, IReqWrite(reqWrite))
+      case RespReadOp(id, respRead) => D.RespReadOp(id, IRespRead(respRead))
+      case RespWriteOp(id, respWrite) => D.RespWriteOp(id, IRespWrite(respWrite))
+      case NoDiskOp => D.NoDiskOp
+    }
+  }
+
+  // Implementation of the state transitions
+
+  /*
+  method handleSync(k: Constants, hs: HeapState, io: DiskIOHandler)
+  returns (success: bool)
+  requires io.initialized()
+  requires Inv(k, hs)
+  modifies HeapSet(hs)
+  modifies io
+  ensures Inv(k, hs)
+  ensures ValidDiskOp(io.diskOp())
+  ensures ADM.M.Next(Ik(k), old(I(k, hs)), I(k, hs),
+    if success then UI.SyncOp else UI.NoOp,
+    IDiskOp(io.diskOp()))
+  // impl defined
+
+  method handleQuery(k: Constants, hs: HeapState, io: DiskIOHandler, key: MS.Key)
+  returns (v: Option<MS.Value>)
+  requires io.initialized()
+  requires Inv(k, hs)
+  modifies HeapSet(hs)
+  modifies io
+  ensures Inv(k, hs)
+  ensures ValidDiskOp(io.diskOp())
+  ensures ADM.M.Next(Ik(k), old(I(k, hs)), I(k, hs),
+    if v.Some? then UI.GetOp(key, v.value) else UI.NoOp,
+    IDiskOp(io.diskOp()))
+  // impl defined
+
+  method handleInsert(k: Constants, hs: HeapState, io: DiskIOHandler, key: MS.Key, value: MS.Value)
+  returns (success: bool)
+  requires io.initialized()
+  requires Inv(k, hs)
+  modifies HeapSet(hs)
+  modifies io
+  ensures Inv(k, hs)
+  ensures ValidDiskOp(io.diskOp())
+  ensures ADM.M.Next(Ik(k), old(I(k, hs)), I(k, hs),
+    if success then UI.PutOp(key, value) else UI.NoOp,
+    IDiskOp(io.diskOp()))
+  // impl defined
+
+
+  // TODO add proof obligation that the InitState together with the initial disk state
+  // from mkfs together refine to the initial state of the BlockCacheSystem.
+
+  function SystemIk(k: ADM.Constants) : CrashSafeMap.Constants
+  function SystemI(k: ADM.Constants, s: ADM.Variables) : CrashSafeMap.Variables
+  requires ADM.Inv(k, s)
+
+  lemma SystemRefinesCrashSafeMapInit(
+    k: ADM.Constants, s: ADM.Variables)
+  requires ADM.Init(k, s)
+  ensures ADM.Inv(k, s)
+  ensures CrashSafeMap.Init(SystemIk(k), SystemI(k, s))
+
+  lemma SystemRefinesCrashSafeMapNext(
+    k: ADM.Constants, s: ADM.Variables, s': ADM.Variables, uiop: ADM.CrashableUIOp)
+  requires ADM.Inv(k, s)
+  requires ADM.Next(k, s, s', uiop)
+  ensures ADM.Inv(k, s')
+  ensures CrashSafeMap.Next(SystemIk(k), SystemI(k, s), SystemI(k, s'), uiop)
+  */
+}
